proof: fixing auxiliary proof files

CoqOfRust/examples/default/examples/ink_contracts/proofs/lib.v
@@ -1,33 +1,44 @@
 Require Import CoqOfRust.CoqOfRust.
 Require Import CoqOfRust.lib.proofs.lib.
-Require Import CoqOfRust.examples.default.examples.ink_contracts.lib.
+Require CoqOfRust.examples.default.examples.ink_contracts.simulations.lib.
+Require CoqOfRust.examples.default.examples.ink_contracts.lib.
 
 Module  Mapping.
 Section Mapping.
   Context {K V : Set}.
   Context (K_eq_neq : forall (k1 k2 : K), k1 = k2 \/ k1 <> k2).
 
-  Axiom get_empty : forall k,
-    Mapping.get (K := K) (V := V) k Mapping.empty =
-    option.Option.None.
+  Axiom get_empty : forall (key : K),
+    simulations.lib.Mapping.get (K := K) (V := V)
+      key
+      simulations.lib.Mapping.empty =
+    None.
 
   (** ** [get]/[insert] rules *)
 
-  Axiom get_insert_eq : forall (k : K) (v : V) m,
-    Mapping.get k (Mapping.insert k v m) = option.Option.Some v.
+  Axiom get_insert_eq : forall (key : K) (v : V) m,
+    simulations.lib.Mapping.get key (simulations.lib.Mapping.insert key v m) =
+    Some v.
 
   Axiom get_insert_neq : forall (k1 k2 : K) (v : V) m,
     k1 <> k2 ->
-    Mapping.get k1 (Mapping.insert k2 v m) = Mapping.get k1 m.
+    simulations.lib.Mapping.get
+      k1
+      (simulations.lib.Mapping.insert k2 v m) =
+    simulations.lib.Mapping.get k1 m.
 
   (** ** [get/equality] rule *)
 
-  Axiom get_all_equal : forall (m1 m2 : Lib.Mapping.t K V),
-    (forall k, Mapping.get k m1 = Mapping.get k m2) ->
+  Axiom get_all_equal : forall (m1 m2 : simulations.lib.Mapping.t K V),
+    (forall k, simulations.lib.Mapping.get k m1 = simulations.lib.Mapping.get k m2) ->
     m1 = m2.
 
   Lemma insert_insert (k : K) (v1 v2 : V) m :
-    Mapping.insert k v2 (Mapping.insert k v1 m) = Mapping.insert k v2 m.
+    simulations.lib.Mapping.insert
+      k
+      v2
+      (simulations.lib.Mapping.insert k v1 m) =
+    simulations.lib.Mapping.insert k v2 m.
   Proof.
     apply get_all_equal; intros k'.
     destruct (K_eq_neq k k') as [H_eq | H_neq].
@@ -38,8 +49,8 @@ Section Mapping.
   Qed.
 
   Lemma insert_id (k : K) (v : V) m :
-    Mapping.get k m = option.Option.Some v ->
-    Mapping.insert k v m = m.
+    simulations.lib.Mapping.get k m = Some v ->
+    simulations.lib.Mapping.insert k v m = m.
   Proof.
     intros H_get.
     apply get_all_equal; intros k'.
@@ -53,8 +64,10 @@ Section Mapping.
 
   Lemma insert_switch (k1 k2 : K) (v1 v2 : V) m :
     k1 <> k2 ->
-    Mapping.insert k1 v1 (Mapping.insert k2 v2 m) =
-    Mapping.insert k2 v2 (Mapping.insert k1 v1 m).
+    simulations.lib.Mapping.insert k1 v1
+      (simulations.lib.Mapping.insert k2 v2 m) =
+    simulations.lib.Mapping.insert k2 v2
+      (simulations.lib.Mapping.insert k1 v1 m).
   Proof.
     intros H_neq.
     apply get_all_equal; intros k'.
@@ -77,25 +90,32 @@ Section Mapping.
   (** ** [sum] rules *)
 
   Axiom sum_empty : forall f,
-    Mapping.sum (K := K) (V := V) f Mapping.empty = 0.
+    simulations.lib.Mapping.sum (K := K) (V := V)
+      f
+      simulations.lib.Mapping.empty =
+    0.
 
   Axiom sum_insert : forall f k v m,
-    Mapping.sum (K := K) (V := V) f (Mapping.insert k v m) =
-      (f v -
-      match Mapping.get k m with
-      | option.Option.None => 0
-      | option.Option.Some v' => f v'
+    simulations.lib.Mapping.sum (K := K) (V := V)
+      f
+      (simulations.lib.Mapping.insert k v m) =
+    (f v -
+      match simulations.lib.Mapping.get k m with
+      | None => 0
+      | Some v' => f v'
       end +
-      Mapping.sum f m)%Z.
+      simulations.lib.Mapping.sum f m)%Z.
 
   (** Forall predicate. *)
   Definition Forall (P : K -> V -> Prop) m : Prop :=
-    forall k v, Mapping.get k m = option.Option.Some v -> P k v.
+    forall k v,
+    simulations.lib.Mapping.get k m = Some v ->
+    P k v.
 
   Lemma Forall_insert : forall P k v m,
     Forall P m ->
     P k v ->
-    Forall P (Mapping.insert k v m).
+    Forall P (simulations.lib.Mapping.insert k v m).
   Proof.
     unfold Forall.
     intros.
