CoqOfRust/lib/proofs/lib.v
@@ -6,7 +6,7 @@ Require CoqOfRust.simulations.M.
 Require Export Lia.
 From Hammer Require Export Tactics.
 
-Import Simulations.M.Notations.
+Import simulations.M.Notations.
 
 (*** Destruct the matched value in an expression [e]. *)
 Ltac destruct_match_in e :=
@@ -33,107 +33,41 @@ Ltac step :=
 
 Module Integer.
   Module Valid.
-    Definition t {A : Set} `{Integer.C A} (v : A) : Prop :=
-      Integer.min <= Integer.to_Z v <= Integer.max.
+    Definition t (kind : Integer.t) (z : Z) : Prop :=
+      Integer.min kind <= z <= Integer.max kind.
   End Valid.
-
-  Module C.
-    Module Valid.
-      Record t (A : Set) `{Integer.C A} : Prop := {
-        to_of_Z z : Integer.to_Z (Integer.of_Z z) = z;
-        of_to_Z v : Integer.of_Z (Integer.to_Z v) = v;
-      }.
-    End Valid.
-
-    Lemma u8_valid : Valid.t u8.t.
-    Proof.
-      sauto lq: on.
-    Qed.
-
-    Lemma u16_valid : Valid.t u16.t.
-    Proof.
-      sauto lq: on.
-    Qed.
-
-    Lemma u32_valid : Valid.t u32.t.
-    Proof.
-      sauto lq: on.
-    Qed.
-
-    Lemma u64_valid : Valid.t u64.t.
-    Proof.
-      sauto lq: on.
-    Qed.
-
-    Lemma u128_valid : Valid.t u128.t.
-    Proof.
-      sauto lq: on.
-    Qed.
-
-    Lemma usize_valid : Valid.t usize.t.
-    Proof.
-      sauto lq: on.
-    Qed.
-
-    Lemma i8_valid : Valid.t i8.t.
-    Proof.
-      sauto lq: on.
-    Qed.
-
-    Lemma i16_valid : Valid.t i16.t.
-    Proof.
-      sauto lq: on.
-    Qed.
-
-    Lemma i32_valid : Valid.t i32.t.
-    Proof.
-      sauto lq: on.
-    Qed.
-
-    Lemma i64_valid : Valid.t i64.t.
-    Proof.
-      sauto lq: on.
-    Qed.
-
-    Lemma i128_valid : Valid.t i128.t.
-    Proof.
-      sauto lq: on.
-    Qed.
-
-    Lemma isize_valid : Valid.t isize.t.
-    Proof.
-      sauto lq: on.
-    Qed.
-  End C.
 End Integer.
 
 Module BinOp.
   Module Error.
-    Lemma add_eq {A : Set} `{Integer.C A} (z1 z2 z : Z) :
-      Integer.C.Valid.t A ->
-      BinOp.Error.add (Integer.of_Z z1) (Integer.of_Z z2) =
-        inl (Integer.of_Z z) ->
+    Lemma add_eq (kind : Integer.t) (z1 z2 z : Z) :
+      BinOp.Error.add (Value.Integer kind z1) (Value.Integer kind z2) =
+        inl (Value.Integer kind z) ->
       z = (z1 + z2)%Z.
     Proof.
       unfold
         BinOp.Error.add,
         BinOp.Error.make_arithmetic,
-        Integer.normalize_error.
+        Integer.normalize_with_error.
       sauto.
     Qed.
 
-    Lemma add_is_valid {A : Set} `{Integer.C A} (v1 v2 v : A)
-      (H_C : Integer.C.Valid.t A)
-      (H_v1 : Integer.Valid.t v1)
-      (H_v2 : Integer.Valid.t v2)
-      (H_v : BinOp.Error.add v1 v2 = inl v) :
-      Integer.Valid.t v.
+    Lemma add_is_valid (kind : Integer.t) (z1 z2 : Z) (v : Value.t)
+      (H_z1 : Integer.Valid.t kind z1)
+      (H_z2 : Integer.Valid.t kind z2)
+      (H_v :
+        BinOp.Error.add (Value.Integer kind z1) (Value.Integer kind z2) =
+          inl v) :
+      match v with
+      | Value.Integer _ z => Integer.Valid.t kind z
+      | _ => False
+      end.
     Proof.
       unfold
         Integer.Valid.t,
         BinOp.Error.add,
         BinOp.Error.make_arithmetic,
-        Integer.normalize_error
+        Integer.normalize_with_error
         in *.
       repeat destruct (_ <? _) eqn:? in H_v; try congruence.
       sauto lq: on solve: lia.
